Write a spec for iteration over a validated buffer
A small sub-part of the proof (that the number of entires parsed from
the beginning of a buffer matches the num_entries from parsing the
entire thing) exposes a fundamental issue with these kinds of lazy
parsing proofs: the parser builds up local state in binds that will end
up in the final result and it would be nice to know this structure
without having to analyze the entire parser.

examples/struct/keyvalue.pos/Test.fst
@@ -324,13 +324,58 @@ let validate =
   admit();
   parse_u32 `then_validate`
   (fun num_entries -> validate_many parse_entry (U32.v num_entries) validate_entry `seq`
-                   validate_done `seq`
-                   validate_accept)
+                   validate_done)
 
 (*! API using validated but unparsed key-value buffer *)
 
 // sufficient to expose iteration over the key-value pairs (specifically pointers to them)
 // TODO: write this in stateful F*; not clear what a useful pure model would be
+
+// spec: fold over fully parsed store
+val fold_left_store: f:('a -> encoded_entry -> 'a) -> 'a -> s:store -> 'a
+let fold_left_store f acc s =
+    let rec aux es acc =
+        match es with
+        | [] -> acc
+        | e::es -> aux es (f acc e) in
+    aux s.entries acc
+
+unfold let optbind (#t:Type) (#t':Type) (x:option t) (f:t -> option t') : option t' =
+  match x with
+  | Some v -> f v
+  | None -> None
+
+val fold_left_buffer: #t:Type -> f:(t -> encoded_entry -> t) -> t -> b:bytes -> t
+let fold_left_buffer #t f acc b =
+    match parse_u32 b with
+    | Some (num_entries, l) -> begin
+       // we only parse up to n more entries from the buffer b
+       let rec aux (n: nat) b acc : t =
+         match n with
+         | 0 -> acc
+         | _ -> begin
+           match parse_entry b with
+           | Some (e, l) ->
+             assert (n > 0);
+             aux (n-1) (slice b l (length b)) (f acc e)
+           | None -> acc
+           end in
+         aux (U32.v num_entries) (slice b l (length b)) acc
+      end
+    | None -> acc
+
+let parse_result (#t:Type) (#b:bytes) (r: option (t * n:nat{n <= length b}){Some? r}) : t = fst (Some?.v r)
+
+// TODO: this is actually a fairly difficult proof: parse_abstract_store does
+// several steps before finally storing the result of the original parse_u32 in
+// num_entries
+assume val parse_num_entries_valid : b:bytes{Some? (validate b)} ->
+  Lemma (parse_u32 b == Some ((parse_result (parse_abstract_store b)).num_entries, 4))
+
+val fold_left_buffer_ok: #t:Type -> f:(t -> encoded_entry -> t) -> acc:t -> b:bytes{Some? (validate b)} ->
+    Lemma (fold_left_buffer f acc b ==
+           fold_left_store f acc (parse_result (parse_abstract_store b)))
+let fold_left_buffer_ok #t f acc b
 
 (*! Parsing a cache *)
 
@@ -343,11 +388,6 @@ let validate =
 // and a proof that the parser + API is the same as the ghost parser (which
 // produces a complete struct) and a ghost API (which might just be field/array
 // accesses)
-
-unfold let optbind (#t:Type) (#t':Type) (x:option t) (f:t -> option t') : option t' =
-  match x with
-  | Some v -> f v
-  | None -> None
 
 let parse_value_offset (b:bytes) : option (n:nat{n <= length b}) =
  parse_u16_array b `optbind`
